update

Coq/Coq32.v
@@ -11,7 +11,120 @@ Load Coq31.
 Module STLCProp.
 Import STLC.
 
+Lemma canonical_forms_bool : ∀t,
+  empty ⊢ t ∈ Bool →
+  value t →
+  (t = tru) ∨ (t = fls).
+Proof.
+  intros t HT HVal.
+  inversion HVal; intros; subst; try inversion HT; auto.
+Qed.
 
+Lemma canonical_forms_fun : ∀t T1 T2,
+  empty ⊢ t ∈ (Arrow T1 T2) →
+  value t →
+  exists x u, t = abs x T1 u.
+Proof.
+  intros t T1 T2 HT HVal.
+  inversion HVal; intros; subst; try inversion HT; subst; auto.
+  exists x0, t0. auto.
+Qed.
+
+Theorem progress : ∀t T,
+  empty ⊢ t ∈ T →
+  value t ∨ ∃t', t -->> t'.
+Proof with eauto.
+  intros t T Ht.
+  remember (@empty ty) as Gamma.
+  induction Ht; subst Gamma...
+  - (* T_Var *)
+    (* contradictory: variables cannot be typed in an
+       empty context *)
+    inversion H.
+  - (* T_App *)
+    (* t = t1 t2.  Proceed by cases on whether t1 is a
+       value or steps... *)
+    right. destruct IHHt1...
+    + (* t1 is a value *)
+      destruct IHHt2...
+      * (* t2 is also a value *)
+        assert (∃x0 t0, t1 = abs x0 T11 t0).
+        eapply canonical_forms_fun; eauto.
+        destruct H1 as [x0 [t0 Heq]]. subst.
+        exists ([x0:=t2]t0)...
+      * (* t2 steps *)
+        inversion H0 as [t2' Hstp]. exists (app t1 t2')...
+    + (* t1 steps *)
+      inversion H as [t1' Hstp]. exists (app t1' t2)...
+  - (* T_Test *)
+    right. destruct IHHt1...
+    + (* t1 is a value *)
+      destruct (canonical_forms_bool t1); subst; eauto.
+    + (* t1 also steps *)
+      inversion H as [t1' Hstp]. exists (test t1' t2 t3)...
+Qed.
+
+Theorem progress' : ∀t T,
+     empty ⊢ t ∈ T →
+     value t ∨ ∃t', t -->> t'.
+Proof with eauto.
+  intros t.
+  induction t; intros T Ht; auto.
+  - inversion Ht;subst. inversion H1.
+  - inversion Ht;subst. right. destruct (IHt1 (Arrow T11 T))...
+    destruct (IHt2 T11)... assert(exists x0 t0, t1 = abs x0 T11 t0). 
+    eapply canonical_forms_fun; eauto. destruct H1 as [x0 [t0 H1]];subst.
+    exists ([x0:=t2]t0)...
+    destruct H0. exists (app t1 x0)... destruct H. exists (app x0 t2)...
+  - right. inversion Ht;subst. destruct (IHt1 Bool)... 
+    destruct (canonical_forms_bool t1); subst; eauto. destruct H. exists (test x0 t2 t3)...
+Qed.
+
+Inductive appears_free_in : string → tm → Prop :=
+  | afi_var : ∀x,
+      appears_free_in x (var x)
+  | afi_app1 : ∀x t1 t2,
+      appears_free_in x t1 →
+      appears_free_in x (app t1 t2)
+  | afi_app2 : ∀x t1 t2,
+      appears_free_in x t2 →
+      appears_free_in x (app t1 t2)
+  | afi_abs : ∀x y T11 t12,
+      y ≠ x →
+      appears_free_in x t12 →
+      appears_free_in x (abs y T11 t12)
+  | afi_test1 : ∀x t1 t2 t3,
+      appears_free_in x t1 →
+      appears_free_in x (test t1 t2 t3)
+  | afi_test2 : ∀x t1 t2 t3,
+      appears_free_in x t2 →
+      appears_free_in x (test t1 t2 t3)
+  | afi_test3 : ∀x t1 t2 t3,
+      appears_free_in x t3 →
+      appears_free_in x (test t1 t2 t3).
+Hint Constructors appears_free_in.
+
+Definition closed (t:tm) :=
+  ∀x, ¬appears_free_in x t.
+
+Lemma free_in_context : ∀x t T Gamma,
+   appears_free_in x t →
+   Gamma ⊢ t ∈ T →
+   ∃T', Gamma x = Some T'.
+Proof.
+  intros x t T Gamma H H0. generalize dependent Gamma.
+  generalize dependent T.
+  induction H;
+         intros; try solve [inversion H0; eauto].
+  - (* afi_abs *)
+    inversion H1; subst.
+    apply IHappears_free_in in H7. unfold update in H7.
+    rewrite t_update_neq in H7; assumption.
+Qed.
+
+Corollary typable_empty__closed : ∀t T,
+    empty ⊢ t ∈ T →
+    closed t.
 
 
 
