Agda/Ag09.agda
@@ -1,3 +1,4 @@
+
 module Ag09 where
 
 import Relation.Binary.PropositionalEquality as Eq
