Agda/JustBeInjective.agda
@@ -1,0 +1,17 @@
+{-# OPTIONS --cubical --safe #-}
+module JustBeInjective where
+
+open import Cubical.Core.Everything
+open import Cubical.Data.Unit
+data maybe (A : Set) : Set where
+  just : A -> maybe A
+  nothing : maybe A
+
+variable A : Set
+
+unwrap : A → (a : maybe A) → A
+unwrap _ (just x) = x
+unwrap a nothing = a
+
+just-injective : ∀ {A : Set} (a b : A) → just a ≡ just b → a ≡ b
+just-injective a b p i = unwrap a (p i)
