Agda/Mod.agda
@@ -1,0 +1,48 @@
+{-# OPTIONS --safe #-}
+module Mod where
+
+open import Data.Fin
+open import Data.Nat as ℕ
+  using (ℕ; zero; suc; z≤n; s≤s)
+open import Relation.Binary.PropositionalEquality
+open import Function
+
+private variable k : ℕ
+
+last : Fin (suc k)
+last {k = zero} = zero
+last {k = suc _} = suc last
+
+negate : Fin k -> Fin k
+negate zero = zero
+negate (suc zero) = last
+negate (suc (suc n)) = inject₁ (negate (suc n))
+
+subt : Fin k -> Fin k -> Fin k
+subt n zero = n
+subt zero (suc m) = negate (suc m)
+subt (suc n) (suc m) with (compare n m)
+...| less _ _ = suc (subt n m)
+...| _ = inject₁ (subt n m)
+
+add : Fin k -> Fin k -> Fin k
+add n m = subt n (negate m)
+
+multAux : ∀{n} → ℕ → (Fin n → Fin n) → Fin n → Fin n
+multAux zero _ x = x
+multAux (suc n) f x = multAux n f (f x)
+
+mult : Fin k -> Fin k -> Fin k
+mult zero m = zero
+mult (suc n) m = multAux (toℕ n) (add m) zero
+
+zer : Fin 5
+zer = zero
+one : Fin 5
+one = suc zero
+two : Fin 5
+two = suc (suc zero)
+three : Fin 5
+three = suc (suc (suc zero))
+four : Fin 5
+four = suc (suc (suc (suc zero)))
