Agda/gugugu.agda
@@ -10,17 +10,21 @@ open import Agda.Builtin.Sigma
 ++-injectiveʳ [] b c p = p
 ++-injectiveʳ (x ∷ a) b c p = ++-injectiveʳ a b c (snd (∷-injective p))
 
--- pretty hard
--- try to use cong to convert to an eazier problem
-
 lemma : ∀ {ℓ} {A : Set ℓ} (x : A) (xs ys : List A) → xs ++ x ∷ ys ≡ (xs ++ x ∷ []) ++ ys
 lemma x [] ys = refl
 lemma x (x₁ ∷ xs) ys = cong (_∷_ x₁) (lemma x xs ys)
 
-silly : ∀ {ℓ} {A : Set ℓ} (x : A) (xs ys : List A) → xs ++ x ∷ [] ≡ ys ++ x ∷ [] → xs ≡ ys
-silly x xs ys p = {!!}
+col : ∀ {ℓ} {A : Set ℓ} (x : A) (xs : List A) → xs ++ x ∷ [] ≡ (xs ∷ʳ x)
+col x [] = refl
+col x (x₁ ∷ xs) = refl
 
+silly' : ∀ {ℓ} {A : Set ℓ} (x : A) (xs ys : List A) → xs ++ x ∷ [] ≡ ys ++ x ∷ [] → xs ∷ʳ x ≡ ys ∷ʳ x
+silly' x xs ys = λ z → z
+
+silly : ∀ {ℓ} {A : Set ℓ} (x : A) (xs ys : List A) → xs ++ x ∷ [] ≡ ys ++ x ∷ [] → xs ≡ ys
+silly x xs ys p rewrite col x xs | col x ys = fst (∷ʳ-injective xs ys (silly' x xs ys p))
+
+-- inductive can do this job too.
 ++-injectiveˡ : ∀ {ℓ} {A : Set ℓ} (a b c : List A) → a ++ c ≡ b ++ c → a ≡ b
 ++-injectiveˡ a b [] p rewrite ++-identityʳ a | ++-identityʳ b = p
 ++-injectiveˡ a b (x ∷ c) p rewrite lemma x a c | lemma x b c = silly x a b (++-injectiveˡ (a ++ x ∷ []) (b ++ x ∷ []) c p)
- 
