Agda/tmp.agda
@@ -15,3 +15,5 @@ lemma x .(x₁ ∷ l) l' (scons x₁ l .(x ∷ l') H) = scons x₁ l l' (lemma x
 less-is-not-more : ∀ {X} x (l : List X) → ¬ Suf l (x ∷ l)
 less-is-not-more x [] = λ ()
 less-is-not-more x (x₁ ∷ l) (scons .x₁ .l .(x ∷ x₁ ∷ l) H) = less-is-not-more x₁ l (lemma x l (x₁ ∷ l) H)
+
+
